Splinter/Journal/Bundle.i.dfy
@@ -1,0 +1,2 @@
+include "../CoordinationLayer/Bundle.i.dfy"
+include "PagedJournalRefinement.i.dfy"
