Splinter/Journal/PagedJournalRefinement.i.dfy
@@ -1,0 +1,113 @@
+// Copyright 2018-2021 VMware, Inc., Microsoft Inc., Carnegie Mellon University, ETH Zurich, and University of Washington
+// SPDX-License-Identifier: BSD-2-Clause
+
+include "PagedJournal.i.dfy"
+
+module PagedJournalRefinement
+// TODO refines RefinementObligation(mapuiop? journaluiop?, AbstractJournal)
+{
+  import opened MsgHistoryMod
+  import opened LSNMod
+  import opened JournalLabels
+  import AbstractJournal
+  import opened PagedJournal
+
+  // The user of this module is probably also going to want a lemma about LoadJournal.
+
+  function I(v: Variables) : (out:AbstractJournal.Variables)
+    requires v.WF()
+    ensures out.WF()
+  {
+    AbstractJournal.Variables(v.I())
+  }
+
+  //////////////////////////////////////////////////////////////////////////////
+  // non-state-machine function & predicate refinement lemmas
+
+  lemma MkfsRefines()
+    ensures Mkfs().I() == AbstractJournal.Mkfs()
+  {
+  }
+
+  lemma SeqEndMatchesRefines(v: Variables, lsn: LSN)
+    requires v.WF()
+    ensures v.SeqEndMatches(lsn) <==> I(v).SeqEndMatches(lsn)
+  {
+  }
+
+  lemma IncludesSubseqRefines(v: Variables, messages: MsgHistory)
+    requires v.WF()
+    requires messages.WF()
+    ensures v.IncludesSubseq(messages) ==> I(v).IncludesSubseq(messages)
+  {
+    if v.IncludesSubseq(messages) {
+      var i:nat :| v.truncatedJournal.IncludesSubseqAt(messages, i);
+      var receipt := v.truncatedJournal.BuildReceiptTJ();
+      receipt.TJFacts();
+
+      // Base case: messages is in the interp of receipt line i
+      assert receipt.OneLinkedInterpretation(i) by { receipt.reveal_LinkedInterpretations(); }
+
+      // now induct forward to the last line
+      while i<|receipt.lines|-1
+        invariant i<|receipt.lines|
+        invariant receipt.lines[i].interpretation.value.WF();
+        invariant receipt.lines[i].interpretation.value.IncludesSubseq(messages);
+      {
+        i := i + 1;
+        assert receipt.OneLinkedInterpretation(i) by { receipt.reveal_LinkedInterpretations(); }
+      }
+    }
+  }
+
+  lemma CanFreezeAsRefines(v: Variables, startLsn: LSN, endLsn: LSN, keepReceiptLines: nat) returns (messages: MsgHistory)
+    requires v.WF()
+    ensures v.CanFreezeAs(startLsn, endLsn, keepReceiptLines) ==> I(v).CanFreezeAs(startLsn, endLsn, messages)
+  {
+    if v.CanFreezeAs(startLsn, endLsn, keepReceiptLines) {
+      if startLsn < endLsn {
+        // endLsn-1 is in the interp, so we can discard to endLsn
+        var i := keepReceiptLines - 1;
+        var receipt := v.truncatedJournal.BuildReceiptTJ();
+        receipt.TJFacts();
+        v.truncatedJournal.SubseqOfEntireInterpretation(receipt.MessageSeqAt(i), i);
+        assert receipt.MessageSeqAt(i).Contains(endLsn-1);  // trigger
+      }
+      messages := I(v).journal.DiscardOld(startLsn).DiscardRecent(endLsn);
+    }
+  }
+
+  //////////////////////////////////////////////////////////////////////////////
+  // State machine refinement
+
+  predicate Inv(v: Variables)
+  {
+    true
+  }
+  
+  lemma InvInit(v: Variables, tj: TruncatedJournal)
+    requires Init(v, tj)
+    ensures Inv(v)
+  {
+  }
+
+  lemma InvNext(v: Variables, v': Variables, lbl: TransitionLabel)
+    requires Inv(v)
+    requires Next(v, v', lbl)
+    ensures Inv(v')
+  {
+  }
+
+  lemma InitRefines(v: Variables, tj: TruncatedJournal)
+    requires Init(v, tj)
+    ensures AbstractJournal.Init(I(v), tj.I())
+  {
+  }
+
+  lemma NextRefines(v: Variables, v': Variables, lbl: TransitionLabel)
+    requires Inv(v)
+    requires Next(v, v', lbl)
+    ensures AbstractJournal.Next(I(v), I(v'), lbl)
+  {
+  }
+} // module
